Loom/Ghost.lean
@@ -1,0 +1,239 @@
+
+
+namespace MathlibErased
+
+/-- `Erased α` is the same as `α`, except that the elements
+  of `Erased α` are erased in the VM in the same way as types
+  and proofs. This can be used to track data without storing it
+  literally. -/
+def Erased (α : Sort u) : Sort max 1 u :=
+  { s : α → Prop // ∃ a, (a = ·) = s }
+
+/-- Erase a value. -/
+@[macro_inline, grind]
+def hide {α} (a : α) : Erased α :=
+  ⟨fun b => a = b, a, rfl⟩
+
+/-- Extracts the erased value, noncomputably. -/
+@[grind]
+noncomputable def Erased.reveal {α} : Erased α → α
+  | ⟨_, h⟩ => Classical.choose h 
+
+
+@[ext, grind ., simp]
+theorem reveal_inj {α} (a b : Erased α) (h : a.reveal  = b.reveal ) : a = b := by
+        unfold Erased.reveal at *
+        grind
+/-
+GhostStateT σ m
+
+x : GST σ m α --> x.erase : m α 
+
+
+WPMonad (GST σ m α) (σ → Pred) EPred
+
+pre : Pred
+
+post : α → σ → Pred
+
+⦃ fun _ => pre ⦄ x ⦃ v, fun _ => post v ⦄
+
+⦃ pre ⦄ x.erase ⦃ v, post v ⦄
+-/
+
+/-- `(>>=)` operation on `Erased`.
+
+This is a separate definition because `α` and `β` can live in different
+universes (the universe is fixed in `Monad`).
+-/
+@[grind]
+def Erased.bind {α β} (a : Erased α) (f : α → Erased β) : Erased β :=
+  ⟨fun b => (f a.reveal).1 b, (f a.reveal).2⟩
+
+@[grind, simp]
+def map {α β} (f : α → β) (a : Erased α) : Erased β :=
+  a.bind (hide ∘ f)
+
+instance instErasedM : Monad Erased where
+  pure := @hide
+  bind := @Erased.bind
+  map := @map
+
+@[simp]
+theorem reveal_hide {α} (a : α) : (hide a : Erased α).reveal = a := by
+  unfold Erased.reveal hide
+  let h : ∃ x, (x = ·) = fun b => a = b := by
+      simp
+  change Classical.choose h = a
+  have hs := Classical.choose_spec h
+  have ht : (Classical.choose h = a) = (a = a) := congrFun hs a
+  exact Eq.mpr ht rfl
+
+@[simp]
+theorem bind_eq {α β} (a : Erased α) (f : α → Erased β) : Erased.bind a f = f a.reveal := by
+  unfold Erased.bind
+  apply Subtype.ext
+  rfl
+
+instance instLawfulMonad : LawfulMonad Erased :=
+  LawfulMonad.mk' Erased
+    (id_map := by
+      intro α x
+      apply reveal_inj
+      simp [Functor.map, map])
+    (pure_bind := by
+      intro α β x f
+      simp [Bind.bind, Pure.pure])
+    (bind_assoc := by
+      intro α β γ x f g
+      simp [Bind.bind])
+
+
+def factorial (n: Nat) : Erased Nat :=
+    if n <= 1 then hide 1
+    else
+        let rest := factorial ( n-1 )
+        hide (n * rest.reveal)
+
+/--
+error: failed to compile definition, consider marking it as 'noncomputable' because it depends on 'Erased.reveal', which is 'noncomputable'
+-/
+#guard_msgs in
+def factorial' (n: Nat) (acc: Nat) : Nat :=
+    if n = 0 then acc
+    else
+        let res := factorial n
+        res.reveal
+
+
+namespace GhostStateCounter
+
+abbrev GhostStateT (σ : Type u) (m : Type u → Type v) (α : Type u) := StateT (Erased σ ) m α
+
+abbrev Counter := Nat
+
+def sumFirstN_Ghost (n: Nat) : GhostStateT Counter Id Nat := do
+    let mut sm := 0
+    for i in [1:n] do
+        let cnt <- get
+        set ( (· + 1) <$> cnt )
+        sm := sm + i
+    pure sm
+
+/- set_option trace.compiler.ir.result true in -/
+def sumFirstN_NoGhost (n: Nat) : Id Nat := do
+    let mut sm := 0
+    for i in [1:n] do
+        sm := sm + i
+    pure sm
+
+theorem sumFirstN_loop_equiv (xs : List Nat) (sm : Nat) (cntr : Erased Counter) :
+    List.foldl (fun b a => b + a) sm xs =
+      (((forIn xs sm fun i r => do
+          let cnt ← get
+          set ((fun x => x + 1) <$> cnt)
+          pure (ForInStep.yield (r + i))) : GhostStateT Counter Id Nat).run cntr).fst := by
+  induction xs generalizing sm cntr with
+  | nil => rfl
+  | cons x xs ih =>
+      simp only [List.foldl, List.forIn_cons]
+      exact ih (sm + x) (((fun x => x + 1) <$> cntr))
+
+theorem equiv : ∀ n cntr, sumFirstN_NoGhost n  =  ((sumFirstN_Ghost n).run cntr).fst := by
+        intros n cntr
+        change Id.run (sumFirstN_NoGhost n) = ((sumFirstN_Ghost n).run cntr).fst
+        simp [sumFirstN_NoGhost, sumFirstN_Ghost]
+        exact sumFirstN_loop_equiv (List.range' 1 (n - 1)) 0 cntr
+
+end GhostStateCounter
+
+end MathlibErased
+
+
+namespace Singleton
+open Lean.Order
+
+def Set (α : Type u) : Type u := α → Prop
+
+def Set.mem (x : α) (s : Set α) : Prop := s x
+
+def Set.mkSingleton (x : α) : Set α := fun y => y = x
+
+inductive Set.IsSingleton (s : Set α) : Prop where
+  | intro (x : α) : (∀ y, s.mem y ↔ y = x) → s.IsSingleton
+
+theorem Set.mk_singleton_is_singleton (x : α) : (Set.mkSingleton x).IsSingleton := by
+  apply Set.IsSingleton.intro x
+  simp [mkSingleton, mem]
+
+structure SingletonSet (α : Type u) where
+  mk' ::
+  toSet : Set α
+  isSingleton : toSet.IsSingleton
+
+def SingletonSet.mk (x : α) : SingletonSet α := ⟨Set.mkSingleton x, Set.mk_singleton_is_singleton x⟩
+
+def SingletonSet.exists_unique (s : SingletonSet α) : ∃ x, ∀ y, s.toSet.mem y ↔ y = x := by
+  rcases s.isSingleton with ⟨x, hx⟩
+  exact ⟨x, hx⟩
+
+noncomputable
+def SingletonSet.get (s : SingletonSet α) : α := s.exists_unique.choose
+
+theorem SingletonSet.mk_get_eq_self (x : α) : (SingletonSet.mk x).get = x := by
+  have h := Classical.choose_spec (SingletonSet.mk x).exists_unique
+  exact ((h x).mp (by simp [SingletonSet.mk, Set.mkSingleton, Set.mem])).symm
+
+theorem SingletonSet.mk_get (s : SingletonSet α) : SingletonSet.mk s.get = s := by
+  cases s with
+  | mk' toSet isSingleton =>
+    unfold SingletonSet.mk
+    congr
+    funext y
+    apply propext
+    have h := Classical.choose_spec (SingletonSet.mk' toSet isSingleton).exists_unique
+    constructor
+    · intro hy
+      exact (h y).mpr hy
+    · intro hy
+      exact (h y).mp hy
+
+-- This is computable unlike `get`!
+def SingletonSet.modify (s : SingletonSet α) (f : α → α) : SingletonSet α :=
+  ⟨fun x => ∃ y, s.toSet.mem y ∧ f y = x,
+  by
+    rcases s.isSingleton with ⟨x, hx⟩
+    apply Set.IsSingleton.intro (f x)
+    intro y
+    constructor
+    · rintro ⟨z, hz, hfz⟩
+      calc
+        y = f z := hfz.symm
+        _ = f x := congrArg f ((hx z).mp hz)
+    · intro hy
+      exact ⟨x, (hx x).mpr rfl, hy.symm⟩ ⟩
+
+theorem SingletonSet.modify_get (s : SingletonSet α) (f : α → α) : (s.modify f).get = f (s.get) := by
+  have hs := Classical.choose_spec s.exists_unique
+  have hmod := Classical.choose_spec (s.modify f).exists_unique
+  have hsget : s.toSet.mem s.get := (hs s.get).mpr rfl
+  exact ((hmod (f s.get)).mp ⟨s.get, hsget, rfl⟩).symm
+
+namespace Credit
+
+abbrev Ghost (α : Type u) : Type u := SingletonSet α
+
+abbrev Credit := Nat
+
+structure CreditT (m : Type u → Type v) (α : Type u) where
+  run : Ghost Credit → m (α × Ghost Credit)
+
+def CreditT.tick [Monad m] : CreditT m Unit :=
+  ⟨fun c => pure (f := m) ((), c.modify (· + 1))⟩
+
+def Credit.default : Ghost Credit := SingletonSet.mk 0
+
+end Credit
+
+
+end Singleton
